QueueingSystems.v
@@ -1,122 +1,333 @@
 Require Import Coq.Lists.List.
 Import ListNotations.
-
+Set Implicit Arguments.
 Require Import DFA.
 
-Require Export Arith_base.
-Require Import BinPos BinInt BinNat Pnat Nnat.
+Require BinIntDef.
 Require Import Omega.
 Local Open Scope Z_scope.
 
-Inductive event {E : Type} : Type :=
-  add | rem | other (e : E).
+Axiom E : Type.
+Inductive event := add | rem | other (e : E).
+Definition E' := event.
+Axiom Q : Type.
+Axiom G : @DFA Q E'.
+Definition q0 := initial_state G.
+Definition pq0 := proper_state q0.
+Definition transition := transition G.
+Definition is_proper_transition q e := exists q',
+  proper_state q' = transition q e.
+Definition xtransition := extended_transition G.
+Definition ixtransition := xtransition pq0.
+Definition generates w := ~ ixtransition w = sink_state.
 
-Definition count_event {E : Type} (e : @event E) : Z :=
+Lemma ixtransition_nil__pq0: ixtransition [] = pq0.
+Proof. auto. Qed.
+
+Lemma extended_transition__transition: forall q e,
+  xtransition (proper_state q) [e] = transition q e.
+Proof. apply DFA.extended_transition__transition. Qed.
+Lemma transition_sink_state: forall w,
+  xtransition sink_state w = sink_state.
+Proof. apply DFA.transition_sink_state. Qed.
+Lemma dist_xtransition: forall w w' q,
+  xtransition q (w ++ w') = xtransition (xtransition q w) w'.
+Proof. apply DFA.dist_extended_transition. Qed.
+Lemma dist_ixtransition: forall w w',
+  ixtransition (w ++ w') = xtransition (ixtransition w) w'.
+Proof. unfold ixtransition. intros w w'. apply dist_xtransition. Qed.
+Theorem prefix_closed: forall w w',
+  generates (w ++ w') -> generates w.
+Proof. apply DFA.prefix_closed. Qed.
+
+Definition count_event (e : E') :=
   match e with
-  add => 1  |
-  rem => -1 |
-  other e' => 0
+    add => 1  |
+    rem => -1 |
+    other e' => 0
   end.
 
-Fixpoint count_buffer {E : Type} (w : list (@event E)) : Z :=
+Fixpoint count_buffer w :=
   match w with
-  [] => 0 |
-  e::w' => count_event e + count_buffer w'
+    [] => 0 |
+    e::w' => count_event e + count_buffer w'
   end.
 
-Definition upper_bound {Q E : Type} (g : dfa Q (@event E)) n0 n :=
-  forall w, g ==> w -> n0 + count_buffer w <= n.
+Lemma dist_count_buffer: forall w1 w2,
+  count_buffer (w1 ++ w2) = count_buffer w1 + count_buffer w2.
+Proof.
+  intros w1 w2.
+  induction w1 as [|e w1 IHw1].
+  - auto.
+  - simpl. rewrite IHw1. omega.
+Qed.
 
-Lemma buffer_change: forall (E : Type) (w : list (@event E)) (e : @event E),
+Lemma dist_count_buffer': forall w e,
   count_buffer (w ++ [e]) = count_buffer w + count_event e.
 Proof.
-  intros E w e.
-  induction w as [|e' w IH].
-  - simpl. omega.
-  - simpl. rewrite IH. omega.
+  intros w e.
+  induction w as [|e' w IH]; simpl; try (rewrite IH); omega.
 Qed.
 
-Lemma buffer_count_leq_f:
-  forall (Q E : Type) (g : dfa Q (@event E)) (f : @state Q->Z) n0,
-    (f(proper_state (initial_state g)) = n0 /\
-      forall (q : Q),
-        f((transition g) q add) >= f(proper_state q) + 1 /\
-        f((transition g) q rem) >= f(proper_state q) - 1 /\
-        (forall (e : E), f((transition g) q (other e)) >= f(proper_state q))
-    ) -> (forall w, g ==> w -> n0 + count_buffer w <= f (extended_transition g (proper_state (initial_state g)) w)).
+Axiom n0 : Z.
+Axiom n : Z.
+
+Definition is_upper_bounded := forall w, generates w -> n0 + count_buffer w <= n.
+
+Definition is_tangible q := exists w,
+  proper_state q = ixtransition w.
+
+Lemma buffer_count_leq_f: forall f,
+  ( f(pq0) = n0 /\ forall q, is_tangible q -> forall e,
+    is_proper_transition q e ->
+      f(transition q e) >= f(proper_state q) + count_event e ) ->
+  forall w, generates w -> n0 + count_buffer w <= f(ixtransition w).
 Proof.
-  intros Q E g f n0 H0 w H2.
-  destruct H0 as [H0 H1].
+  intros f [H H0] w H1.
   induction w as [|e w IHw] using @rev_ind.
-  - simpl. omega.
-  - assert (H3 : g ==> w).
-    { apply prefix_closed in H2. apply H2. }
-    apply IHw in H3.
-    rewrite dist_extended_transition.
-    rewrite buffer_change.
-    remember (extended_transition g (proper_state (initial_state g)) w) as q eqn:eq_q. destruct q.
-    + apply prefix_closed in H2. unfold generated_by in H2. unfold not in H2. symmetry in eq_q. apply H2 in eq_q. destruct eq_q.
-    + rewrite extended_transition__transition. assert (f (transition g q e) >= f (proper_state q) + count_event e).
-      { destruct e.
-        - simpl. apply H1.
-        - simpl. apply H1.
-        - simpl. replace (f (proper_state q) + 0) with (f (proper_state q)). apply H1. omega. }
+  - simpl.
+    rewrite ixtransition_nil__pq0.
+    omega.
+  - pose H1 as H2; apply prefix_closed in H2.
+    apply IHw in H2.
+    rewrite dist_ixtransition.
+    rewrite dist_count_buffer'.
+    remember (ixtransition w) as q eqn:eq_q.
+    destruct q.
+    {
+      apply prefix_closed in H1.
+      unfold generates in H1.
+      symmetry in eq_q.
+      contradiction.
+    }
+    remember (xtransition (proper_state q) [e]) as q' eqn:eq_q'; destruct q' as [|q'].
+    + unfold generates in H1; rewrite dist_ixtransition in H1.
+      symmetry in eq_q'.
+      rewrite eq_q in eq_q'.
+      contradiction.
+    + assert (H3: proper_state q' = transition q e).
+      { rewrite extended_transition__transition in eq_q'; auto. }
+      assert (f (proper_state q') >= f (proper_state q) + count_event e).
+      {
+        rewrite H3.
+        apply H0.
+        - exists w. auto.
+        - exists q'. auto.
+      }
+      omega.
+Qed.
+
+Theorem upper_bound1:
+  ( exists f, f(pq0) = n0 /\ forall q, is_tangible q ->
+    f(proper_state q) <= n /\ ( forall e, is_proper_transition q e ->
+      f(transition q e) >= f(proper_state q) + count_event e ) ) ->
+  is_upper_bounded.
+Proof.
+  unfold is_upper_bounded.
+  intros [f [H H0]] w H1.
+  assert (H2: n0 + count_buffer w <= f(ixtransition w)).
+  { apply buffer_count_leq_f; try split; try (apply H0); auto. }
+  assert (f (ixtransition w) <= n).
+  {
+    destruct (ixtransition w) as [|q] eqn:eq.
+    - contradiction.
+    - destruct H0 with (q:=q); try (exists w); auto.
+  }
+  omega.
+Qed.
+
+Notation " w ~> q " := (ixtransition w = q) (at level 60).
+
+Lemma g2__generates: forall w q,
+  w ~> (proper_state q) -> generates w.
+Proof.
+  unfold generates, not.
+  intros w q H H0.
+  rewrite H in H0.
+  discriminate.
+Qed.
+
+Lemma not_nil_if_count: forall w,
+  count_buffer w > 0 -> w <> [].
+Proof.
+  unfold not.
+  intros w H H0.
+  destruct w.
+  - inversion H.
+  - discriminate.
+Qed.
+
+Lemma cycle: forall q,
+  forall w, xtransition q w = q -> xtransition q (w++w) = q.
+Proof.
+  intros q w H.
+  rewrite dist_xtransition.
+  rewrite H.
+  auto.
+Qed.
+
+Fixpoint word_pow (w:list E') (n:nat) :=
+  match n with
+    O => [] |
+    S n => w ++ (word_pow w n)
+  end.
+
+Theorem count_word_pow: forall w n,
+  count_buffer (word_pow w n) = (Z.of_nat n) * (count_buffer w).
+Proof.
+  intros w n.
+  induction n as [|n IHn].
+  - auto.
+  - replace (word_pow w (S n)) with (w ++ word_pow w n).
+    rewrite dist_count_buffer.
+    rewrite IHn.
+    rewrite Nat2Z.inj_succ, <- Zmult_succ_l_reverse.
+    omega.
+    auto.
+Qed.
+
+Lemma q0_cycle: forall w n,
+  w ~> pq0 -> (word_pow w n) ~> pq0.
+Proof.
+  intros w n H.
+  induction n as [|n IHn].
+  - auto.
+  - simpl.
+    rewrite dist_ixtransition.
+    rewrite H.
+    auto.
+Qed.
+
+Lemma q0_cycle_count: forall w n,
+  (count_buffer w > 0 /\ w ~> pq0) ->
+  exists w', w' ~> pq0 /\ count_buffer w' > n.
+Proof.
+  intros w n [H H0].
+  destruct n eqn:eq_n.
+  - exists w. auto.
+  - exists (word_pow w ((Pos.to_nat p)+1)).
+    split.
+    + apply q0_cycle.
+      auto.
+    + rewrite count_word_pow.
+      assert (Z.pos p > 0). { apply Zgt_pos_0. }
+      assert (Z.pos p + 1 <= Z.of_nat (Pos.to_nat p + 1) * count_buffer w).
+      {
+        replace (Z.pos p + 1) with ((Z.pos p + 1)*1); try omega.
+        apply Zmult_le_compat; try omega.
+        rewrite Z.add_1_r. replace ((Pos.to_nat p + 1)%nat) with ((S (Pos.to_nat p))); try omega.
+        simpl.
+        rewrite Zpos_P_of_succ_nat.
+        rewrite positive_nat_Z.
+        simpl.
+        omega.
+      }
+      omega.
+  - exists w.
+    split.
+    + auto.
+    + rewrite <- eq_n.
+      assert (n < 0). { rewrite eq_n. apply Zlt_neg_0. }
+      omega.
+Qed.
+
+Lemma q0_cycle_no_upper_bound:
+  (exists w, w ~> pq0 /\ count_buffer w > 0) -> ~ is_upper_bounded.
+Proof.
+  unfold is_upper_bounded, not.
+  intros [w [H H0]] H1.
+  assert (H2: count_buffer w > 0 /\ w ~> pq0). auto.
+  apply q0_cycle_count with(n:=(n-n0)) in H2.
+  destruct H2 as [w' [H2 H3]].
+  apply g2__generates, H1 in H2.
+  omega.
+Qed.
+
+Definition state_upper_bound q m :=
+  forall w, w ~> q -> n0 + count_buffer w <= m.
+
+Definition min_state_upper_bound q m :=
+  state_upper_bound q m /\ ~ state_upper_bound q (m-1).
+
+Theorem q0_n0_bounded: is_upper_bounded -> min_state_upper_bound pq0 n0.
+Proof.
+  unfold min_state_upper_bound, state_upper_bound.
+  intro H.
+  split.
+  - intros w H0.
+    destruct (count_buffer w) eqn:eq_count.
+    + omega.
+    + assert (count_buffer w > 0). { rewrite eq_count. apply Zgt_pos_0. }
+      assert (exists w, w ~> pq0 /\ count_buffer w > 0). { exists w. auto. }
+      apply q0_cycle_no_upper_bound in H2.
+      contradiction.
+    + assert (Z.neg p < 0). { apply Zlt_neg_0. }
+      omega.
+  - unfold not. intro H0.
+    assert (H1: [] ~> pq0). { auto. }
+    apply H0 in H1.
+    simpl in H1.
     omega.
 Qed.
 
-Theorem th1:
-  forall (Q E : Type) (g : dfa Q (@event E)) n0 n,
-    (exists (f : @state Q->Z), f(proper_state (initial_state g)) = n0 /\
-      forall (q : Q),
-        f(proper_state q) <= n /\
-        f((transition g) q add) >= f(proper_state q) + 1 /\
-        f((transition g) q rem) >= f(proper_state q) - 1 /\
-        (forall (e : E), f((transition g) q (other e)) >= f(proper_state q))
-    ) -> upper_bound g n0 n.
+Lemma transition_upper_bound: forall q m1 m2 e,
+  is_tangible q -> min_state_upper_bound (proper_state q) m1 ->
+  min_state_upper_bound (transition q e) m1 -> m2 >= m1 + count_event e.
 Proof.
-  unfold upper_bound.
-  intros Q E g n0 n H0 w H2.
-  destruct H0 as [f [H0 H1]].
-  assert (H3: n0 + count_buffer w <= f (extended_transition g (proper_state (initial_state g)) w)).
-  { apply buffer_count_leq_f.
-      - split.
-        + apply H0.
-        + intros H3. apply H1.
-      - apply H2. }
-  remember (extended_transition g (proper_state (initial_state g)) w) as q eqn:eq_q.
-  destruct q.
-  - unfold generated_by in H2. unfold not in H2. symmetry in eq_q. apply H2 in eq_q.
-    destruct eq_q.
-  - assert (f (proper_state q) <= n).
-    { apply H1. }
-    omega.
-Qed.
-
-Theorem th2:
-  forall (Q E : Type) (g : dfa Q (@event E)) n0 n,
-    upper_bound g n0 n ->
-    (exists (f : @state Q->Z), f(proper_state (initial_state g)) = n0 /\
-      forall (q : Q),
-        f(proper_state q) <= n /\
-        f((transition g) q add) >= f(proper_state q) + 1 /\
-        f((transition g) q rem) >= f(proper_state q) - 1 /\
-        (forall (e : E), f((transition g) q (other e)) >= f(proper_state q))
-    ).
-Proof.
-(* FICA PARA O TCC 2 ;-) *)
 Admitted.
 
-Theorem th12:
-  forall (Q E : Type) (g : dfa Q (@event E)) n0 n,
-    (exists (f : @state Q->Z), f(proper_state (initial_state g)) = n0 /\
-      forall (q : Q),
-        f(proper_state q) <= n /\
-        f((transition g) q add) >= f(proper_state q) + 1 /\
-        f((transition g) q rem) >= f(proper_state q) - 1 /\
-        (forall (e : E), f((transition g) q (other e)) >= f(proper_state q))
-    ) <-> upper_bound g n0 n.
+Axiom func_choice : forall A B (R : A -> B -> Prop),
+  (forall x, exists y, R x y) -> exists f, forall x, R x (f x).
+
+Definition f_prop pq m := forall q,
+  pq = proper_state q -> is_tangible q -> min_state_upper_bound pq m.
+
+Lemma f_def:
+  is_upper_bounded -> exists f, forall q, f_prop q (f q).
 Proof.
+  intro H.
+  apply func_choice.
+  unfold f_prop.
+  intro q.
+Admitted.
+
+Lemma f_unicity: forall q m1 m2,
+  min_state_upper_bound q m1 -> min_state_upper_bound q m2 -> m1 = m2.
+Proof.
+Admitted.
+
+Theorem upper_bound2:
+  is_upper_bounded ->
+  ( exists f, f(pq0) = n0 /\ forall q, is_tangible q ->
+    f(proper_state q) <= n /\ ( forall e, is_proper_transition q e ->
+      f(transition q e) >= f(proper_state q) + count_event e ) ).
+Proof.
+  intro H.
+  pose H as H0; apply f_def in H0; destruct H0 as [f H0].
+  unfold f_prop in H0.
+  exists f.
   split.
-  apply th1.
-  apply th2.
+  - destruct H0 with (q:=pq0) (q0:=q0); try (exists []); auto.
+    apply q0_n0_bounded in H.
+    apply f_unicity with (q:=pq0); unfold min_state_upper_bound; auto.
+  - intros q H1.
+    split.
+    + 
+Admitted.
+
+Theorem upper_bound:
+  ( exists f, f(pq0) = n0 /\ forall q, is_tangible q ->
+    f(proper_state q) <= n /\ ( forall e, is_proper_transition q e ->
+      f(transition q e) >= f(proper_state q) + count_event e ) ) <->
+  is_upper_bounded.
+Proof.
+  split. apply upper_bound1. apply upper_bound2.
 Qed.
+
+
+
+
+
+
+
+
